hax-lib/macros/src/utils.rs
@@ -1,23 +1,12 @@
 use crate::prelude::*;
 use crate::rewrite_self::*;
 
-/// `HaxQuantifiers` expands to the definition of the `forall` and `exists` functions
+/// `HaxQuantifiers` makes polymorphic expression inlining functions available
 pub struct HaxQuantifiers;
 impl ToTokens for HaxQuantifiers {
     fn to_tokens(&self, tokens: &mut proc_macro2::TokenStream) {
         let status_attr = &AttrPayload::ItemStatus(ItemStatus::Included { late_skip: true });
         quote! {
-            #AttrHaxLang
-            #status_attr
-            fn forall<T, U:Into<hax_lib::Prop>, F: Fn(T) -> U>(f: F) -> hax_lib::Prop {
-                true.into()
-            }
-            #AttrHaxLang
-            #status_attr
-            fn exists<T, U:Into<hax_lib::Prop>, F: Fn(T) -> U>(f: F) -> hax_lib::Prop {
-                true.into()
-            }
-
             use ::hax_lib::fstar_unsafe_expr as fstar;
             use ::hax_lib::coq_unsafe_expr as coq;
             use ::hax_lib::proverif_unsafe_expr as proverif;
@@ -279,7 +268,7 @@ pub fn make_fn_decoration(
             sig.output = if let FnDecorationKind::Decreases = &kind {
                 syn::parse_quote! { -> Box<dyn Any> }
             } else {
-                syn::parse_quote! { -> impl Into<hax_lib::Prop> }
+                syn::parse_quote! { -> impl Into<::hax_lib::Prop> }
             };
             sig
         };
