hax-lib/proofs/fstar/extraction/Hax_lib.fst
@@ -2,13 +2,8 @@ module Hax_lib
 #set-options "--fuel 0 --ifuel 1 --z3rlimit 15"
 open FStar.Tactics
 
-val v_assert (p: bool) : Pure unit (requires p) (ensures (fun x -> p))
-let v_assert (v__formula: bool) = ()
+val v_assert (p: Type0) : Pure unit (requires p) (ensures (fun x -> p))
+let v_assert (v__formula: Type0) = ()
 
-val v_assume (p: bool) : Pure unit (requires True) (ensures (fun x -> p))
-let v_assume (v__formula: bool) = assume v__formula
-
-
-unfold let v_exists (v__f: 'a -> t_Prop): t_Prop = exists (x: 'a). v__f x
-unfold let v_forall (v__f: 'a -> t_Prop): t_Prop = forall (x: 'a). v__f x
-unfold let implies (lhs: t_Prop) (rhs: (x:unit{lhs} -> t_Prop)): t_Prop = (~ lhs) \/ rhs ()
+val v_assume (p: Type0) : Pure unit (requires True) (ensures (fun x -> p))
+let v_assume (v__formula: Type0) = assume v__formula
